Define partial behavior

src/lang/Behavior.v
@@ -35,32 +35,36 @@ Set Implicit Arguments.
 
 Inductive behaviors
           (step: forall (e:MachineEvent.t) (tid:Ident.t) (c1 c2:Configuration.t), Prop):
-  forall (conf:Configuration.t) (b:list Event.t), Prop :=
+  forall (conf:Configuration.t) (b:list Event.t) (f: bool), Prop :=
 | behaviors_nil
     c
     (TERMINAL: Configuration.is_terminal c):
-    behaviors step c nil
+    behaviors step c nil true
 | behaviors_syscall
-    e tid c1 c2 beh
-    (STEP: step (MachineEvent.syscall e) tid c1 c2)
-    (NEXT: behaviors step c2 beh):
-    behaviors step c1 (e::beh)
+    e1 e2 tid c1 c2 beh f
+    (STEP: step (MachineEvent.syscall e2) tid c1 c2)
+    (NEXT: behaviors step c2 beh f)
+    (EVENT: Event.le e1 e2):
+    behaviors step c1 (e1::beh) f
 | behaviors_failure
-    tid c1 c2 beh
+    tid c1 c2 beh f
     (STEP: step MachineEvent.failure tid c1 c2):
-    behaviors step c1 beh
+    behaviors step c1 beh f
 | behaviors_tau
-    tid c1 c2 beh
+    tid c1 c2 beh f
     (STEP: step MachineEvent.silent tid c1 c2)
-    (NEXT: behaviors step c2 beh):
-    behaviors step c1 beh
+    (NEXT: behaviors step c2 beh f):
+    behaviors step c1 beh f
+| behaviors_partial_term
+    c:
+    behaviors step c [] false
 .
 
 Lemma rtc_tau_step_behavior
-      step c1 c2 b
+      step c1 c2 b f
       (STEPS: rtc (union (step MachineEvent.silent)) c1 c2)
-      (BEH: behaviors step c2 b):
-  behaviors step c1 b.
+      (BEH: behaviors step c2 b f):
+  behaviors step c1 b f.
 Proof.
   revert BEH. induction STEPS; auto. inv H.
   i. specialize (IHSTEPS BEH). econs 4; eauto.
@@ -69,13 +73,14 @@ Qed.
 Lemma le_step_behavior_improve
       sem0 sem1
       (STEPLE: sem0 <4= sem1):
-  behaviors sem0 <2= behaviors sem1.
+  behaviors sem0 <3= behaviors sem1.
 Proof.
   i. ginduction PR; i.
   - econs 1; eauto.
   - econs 2; eauto.
   - econs 3; eauto.
   - econs 4; eauto.
+  - econs 5; eauto.
 Qed.
 
 Inductive behaviors_partial
@@ -120,14 +125,14 @@ Proof.
 Qed.
 
 Lemma behaviors_partial_app
-      step c1 c2 b1 b2
+      step c1 c2 b1 b2 f
       (BEH1: behaviors_partial step c1 c2 b1)
-      (BEH2: behaviors step c2 b2)
+      (BEH2: behaviors step c2 b2 f)
   :
-    behaviors step c1 (b1 ++ b2).
+    behaviors step c1 (b1 ++ b2) f.
 Proof.
   induction BEH1.
   - eauto.
-  - econs 2; eauto.
+  - econs 2; eauto. refl.
   - econs 4; eauto.
 Qed.
